@prefix skos: <http://www.w3.org/2004/02/skos/core#> . 
@prefix rdfs: <http://www.w3.org/2000/01/rdf-schema#> .
@prefix reg:  <http://purl.org/linked-data/registry#> .
@prefix dct:  <http://purl.org/dc/terms/> . 

<http://codes.wmo.int/49-2/observable-property/AIRMETEvolvingConditionCollectionAnalysis>
	a skos:Concept ;
	dct:description "The set of physical properties evaluated as a result of an AIRMET, as specified in Technical Regulations, Volume II (WMO-No. 49): Meteorological Services for International Air Navigation." ;
	rdfs:label "AIRMET Evolving Condition Collection Analysis" ;
	skos:notation "AIRMETEvolvingConditionCollectionAnalysis" ;
	reg:status "experimental" ;
	reg:related "" .

<http://codes.wmo.int/49-2/observable-property/MeteorologicalAerodromeForecast>
	a skos:Concept ;
	dct:description "The set of physical properties evaluated as a result of an aerodrome forecast (TAF), as specified in the Technical Regulations (WMO-No. 49), Volume II – Meteorological Service for International Air Navigation." ;
	rdfs:label "Meteorological aerodrome forecast" ;
	skos:notation "MeteorologicalAerodromeForecast" ;
	reg:status "stable" ;
	reg:related "http://codes.wmo.int/ui/resources/observableProperty_MeteorologicalAerodromeForecast.xml" .

<http://codes.wmo.int/49-2/observable-property/MeteorologicalAerodromeObservation>
	a skos:Concept ;
	dct:description "The set of physical properties evaluated as a result of the observation procedure of a routine or special aerodrome meteorological report (METAR or SPECI), as specified in the Technical Regulations (WMO-No. 49), Volume II – Meteorological Service for International Air Navigation." ;
	rdfs:label "Meteorological aerodrome observation" ;
	skos:notation "MeteorologicalAerodromeObservation" ;
	reg:status "stable" ;
	reg:related "http://codes.wmo.int/ui/resources/observableProperty_MeteorologicalAerodromeObservation.xml" .

<http://codes.wmo.int/49-2/observable-property/MeteorologicalAerodromeTrendForecast>
	a skos:Concept ;
	dct:description "The set of physical properties evaluated as a result of the trend forecast procedure of a routine or special aerodrome meteorological report (METAR or SPECI), as specified in the Technical Regulations (WMO-No. 49), Volume II – Meteorological Service for International Air Navigation." ;
	rdfs:label "Meteorological aerodrome trend forecast" ;
	skos:notation "MeteorologicalAerodromeTrendForecast" ;
	reg:status "stable" ;
	reg:related "http://codes.wmo.int/ui/resources/observableProperty_MeteorologicalAerodromeTrendForecast.xml" .

<http://codes.wmo.int/49-2/observable-property/SIGMETEvolvingConditionCollectionAnalysis>
	a skos:Concept ;
	dct:description "The set of meteorological conditions  to be reported in a SIGMET, as specified in Technical Regulations, Volume II (WMO-No. 49): Meteorological Services for International Air Navigation." ;
	rdfs:label "SIGMET Evolving Condition Collection Analysis" ;
	skos:notation "SIGMETEvolvingConditionCollectionAnalysis" ;
	reg:status "experimental" ;
	reg:related "" .

<http://codes.wmo.int/49-2/observable-property/SIGMETPositionCollectionAnalysis>
	a skos:Concept ;
	dct:description "The set of locations where meteorological conditions exist to be reported in a SIGMET, as specified in Technical Regulations, Volume II (WMO-No. 49): Meteorological Services for International Air Navigation." ;
	rdfs:label "SIGMET Position Collection Analysis" ;
	skos:notation "SIGMETPositionCollectionAnalysis" ;
	reg:status "experimental" ;
	reg:related "" .
