@prefix skos: <http://www.w3.org/2004/02/skos/core#> . 
@prefix rdfs: <http://www.w3.org/2000/01/rdf-schema#> .
@prefix reg:  <http://purl.org/linked-data/registry#> .
@prefix dct:  <http://purl.org/dc/terms/> . 

<http://codes.wmo.int/49-2/SpaceWxPhenomena/GNSS_MOD>
	a skos:Concept ;
	dct:description "GNSS-based navigation and surveillance (degradation) - moderate" ;
	rdfs:label "GNSS-based navigation and surveillance (degradation) - moderate" ;
	skos:notation "GNSS_MOD" ;
	reg:status "stable" ;
	reg:related "" .

<http://codes.wmo.int/49-2/SpaceWxPhenomena/GNSS_SEV>
	a skos:Concept ;
	dct:description "GNSS-based navigation and surveillance (degradation) - severe" ;
	rdfs:label "GNSS-based navigation and surveillance (degradation) - severe" ;
	skos:notation "GNSS_SEV" ;
	reg:status "stable" ;
	reg:related "" .

<http://codes.wmo.int/49-2/SpaceWxPhenomena/HF_COM_MOD>
	a skos:Concept ;
	dct:description "HF communications (propagation, absorption) - moderate" ;
	rdfs:label "HF communications (propagation, absorption) - moderate" ;
	skos:notation "HF_COM_MOD" ;
	reg:status "stable" ;
	reg:related "" .

<http://codes.wmo.int/49-2/SpaceWxPhenomena/HF_COM_SEV>
	a skos:Concept ;
	dct:description "HF communications (propagation, absorption) - severe" ;
	rdfs:label "HF communications (propagation, absorption) - severe" ;
	skos:notation "HF_COM_SEV" ;
	reg:status "stable" ;
	reg:related "" .

<http://codes.wmo.int/49-2/SpaceWxPhenomena/RADIATION_MOD>
	a skos:Concept ;
	dct:description "Radiation at flight levels (increased exposure) - moderate" ;
	rdfs:label "Radiation at flight levels (increased exposure) - moderate" ;
	skos:notation "RADIATION_MOD" ;
	reg:status "stable" ;
	reg:related "" .

<http://codes.wmo.int/49-2/SpaceWxPhenomena/RADIATION_SEV>
	a skos:Concept ;
	dct:description "Radiation at flight levels (increased exposure) - severe" ;
	rdfs:label "Radiation at flight levels (increased exposure) - severe" ;
	skos:notation "RADIATION_SEV" ;
	reg:status "stable" ;
	reg:related "" .

<http://codes.wmo.int/49-2/SpaceWxPhenomena/SATCOM_MOD>
	a skos:Concept ;
	dct:description "Communications via satellite (propagation, absorption) - moderate" ;
	rdfs:label "Communications via satellite (propagation, absorption) - moderate" ;
	skos:notation "SATCOM_MOD" ;
	reg:status "stable" ;
	reg:related "" .

<http://codes.wmo.int/49-2/SpaceWxPhenomena/SATCOM_SEV>
	a skos:Concept ;
	dct:description "Communications via satellite (propagation, absorption) - severe" ;
	rdfs:label "Communications via satellite (propagation, absorption) - severe" ;
	skos:notation "SATCOM_SEV" ;
	reg:status "stable" ;
	reg:related "" .
