@prefix skos: <http://www.w3.org/2004/02/skos/core#> . 
@prefix rdfs: <http://www.w3.org/2000/01/rdf-schema#> .
@prefix reg:  <http://purl.org/linked-data/registry#> .
@prefix dct:  <http://purl.org/dc/terms/> . 

<http://codes.wmo.int/49-2/SpaceWxLocation/DAYLIGHT_SIDE>
	a skos:Concept ;
	dct:description "Daylight Side" ;
	rdfs:label "Daylight Side" ;
	skos:notation "DAYLIGHT_SIDE" ;
	reg:status "stable" ;
	reg:related "" .

<http://codes.wmo.int/49-2/SpaceWxLocation/EQN>
	a skos:Concept ;
	dct:description "Equatorial latitudes northern hemisphere (30\u00B0N - 0\u00B0N)" ;
	rdfs:label "Equatorial latitudes northern hemisphere" ;
	skos:notation "EQN" ;
	reg:status "stable" ;
	reg:related "" .

<http://codes.wmo.int/49-2/SpaceWxLocation/EQS>
	a skos:Concept ;
	dct:description "Equatorial latitudes southern hemisphere (0\u00B0S - 30\u00B0S)" ;
	rdfs:label "Equatorial latitudes southern hemisphere" ;
	skos:notation "EQS" ;
	reg:status "stable" ;
	reg:related "" .

<http://codes.wmo.int/49-2/SpaceWxLocation/HNH>
	a skos:Concept ;
	dct:description "High latitudes northern hemisphere (90\u00B0N - 60\u00B0N)" ;
	rdfs:label "High latitudes northern hemisphere" ;
	skos:notation "HNH" ;
	reg:status "stable" ;
	reg:related "" .

<http://codes.wmo.int/49-2/SpaceWxLocation/HSH>
	a skos:Concept ;
	dct:description "High latitudes southern hemisphere (60\u00B0S - 90\u00B0S)" ;
	rdfs:label "High latitudes southern hemisphere" ;
	skos:notation "HSH" ;
	reg:status "stable" ;
	reg:related "" .

<http://codes.wmo.int/49-2/SpaceWxLocation/MNH>
	a skos:Concept ;
	dct:description "Middle latitudes northern hemisphere (60\u00B0N - 30\u00B0N)" ;
	rdfs:label "Middle latitudes northern hemisphere" ;
	skos:notation "MNH" ;
	reg:status "stable" ;
	reg:related "" .

<http://codes.wmo.int/49-2/SpaceWxLocation/MSH>
	a skos:Concept ;
	dct:description "Middle latitudes southern hemisphere (30\u00B0S - 60\u00B0S)" ;
	rdfs:label "Middle latitudes southern hemisphere" ;
	skos:notation "MSH" ;
	reg:status "stable" ;
	reg:related "" .
